1. verif_Is_from is done, with comments explaining the admits. It appears we need an extension in CompCert. 2. Using new gc.v in consultation with Shengyi and Qinxiang. 3. The new gather_SEP takes patterns instead of numerical arguments. Edited our code to cut down on warnings about this. Found a bug in the new gather_SEP, and reported this bug to VST/issues.

CertiGC/verif_Is_from.v
@@ -1,5 +1,17 @@
+(******************************)
+(*                            *)
+(*          CONTENTS          *)
+(*                            *)
+(* is_from          line  14  *)
+(* int_or_ptr, v1   line 275  *)
+(* int_or_ptr, v2   line 350  *) 
+(*                            *)
+(******************************)
+
 Require Export compcert.common.Events.
-Require Export RamifyCoq.CertiGC.gc_spec.
+Require Export RamifyCoq.CertiGC.gc_spec. (** sadly, we do need this import *)
+
+(* Verification of the function Is_from *)
 
 Definition valid_block (m : mem) (b : block) (o : ptrofs) (n : Z) : Prop :=
   0 < n /\
@@ -12,15 +24,16 @@ Definition Is_from_sem : extcall_sem :=
     m1 = m2 /\ trc = nil /\ 
     match args with
     | (Vptr b1 o1) :: (Vptr b2 o2) :: (Vptr b3 o3) :: nil =>
-      exists n : Z, 0 < n /\ Ptrofs.unsigned o1 + n < Int.modulus /\
-                    (b1 = b2) /\ (Ptrofs.unsigned o1 + n = Ptrofs.unsigned o2) /\
+      exists n : Z, 0 < n /\
+                    Ptrofs.unsigned o1 + n < Int.modulus /\
+                    b1 = b2 /\
+                    Ptrofs.unsigned o1 + n = Ptrofs.unsigned o2 /\
                     valid_block m1 b1 o1 n /\
                     common.Memory.Mem.valid_pointer m1 b3 (Ptrofs.unsigned o3) = true /\
-                    ((b1 = b3 /\ (Ptrofs.unsigned o1 <=
-                                  Ptrofs.unsigned o3 <
-                                  Ptrofs.unsigned o2)
-                      /\ ret = Vone) \/
-                     (((b1 <> b3) \/
+                    ((b1 = b3 /\
+                      Ptrofs.unsigned o1 <= Ptrofs.unsigned o3 < Ptrofs.unsigned o2 /\
+                      ret = Vone) \/
+                     ((b1 <> b3 \/
                        (b1 = b3 /\
                         (Ptrofs.unsigned o3 < Ptrofs.unsigned o1 \/
                          Ptrofs.unsigned o3 >= Ptrofs.unsigned o2)))
@@ -52,16 +65,16 @@ Qed.
 
 Lemma Is_from_extcall: extcall_properties Is_from_sem Is_from_sig.
 Proof.
-  constructor.
-  - intros. destruct H as [_ [_ ?]].
+  constructor; intros.
+  - destruct H as [_ [_ ?]].
     do 4 (destruct vargs; try destruct v; try contradiction).
     destruct H as [_ [_ [_ [_ [_ [_ [_ ?]]]]]]].
     destruct H as [[_ [_ ?]] | [_ ?]]; subst; apply I.
-  - intros; apply H0.
-  - intros. destruct H as [? _]. subst m1. trivial. 
-  - intros. destruct H as [? _]. subst m1. trivial. 
-  - intros. destruct H as [? _]. subst m1; apply Mem.unchanged_on_refl.
-  - intros. exists vres, m1'.
+  - apply H0.
+  - destruct H as [? _]. subst m1. trivial. 
+  - destruct H as [? _]. subst m1. trivial. 
+  - destruct H as [? _]. subst m1; apply Mem.unchanged_on_refl.
+  - exists vres, m1'.
     destruct H as [? [? ?]]; subst m2 t.
     split.      
     2: split3; [apply Val.lessdef_refl | trivial | apply Mem.unchanged_on_refl].
@@ -73,9 +86,9 @@ Proof.
     destruct H3 as [n [? [? [? [? ?]]]]].
     exists n. do 4 (split; trivial).
     clear -H0 H4. destruct H4 as [? [? ?]].
-    split3; [apply (mem_ext_valid_block _ _ _ _ _ H0 H) | eapply Mem.valid_pointer_extends; eauto | tauto].
-  - intros. exists f, vres, m1'. destruct H0 as [? [? ?]]. 
-    split.
+    split3; [apply (mem_ext_valid_block _ _ _ _ _ H0 H) |
+             eapply Mem.valid_pointer_extends; eauto | tauto].
+  - intros. exists f, vres, m1'. destruct H0 as [? [? ?]]. split.
     2: {
       split.
       - clear -H4.
@@ -107,8 +120,7 @@ Proof.
         rewrite Z.add_mod_idemp_r, Z.mod_small by easy. omega.
       }
       clear -Hx Hy Hf H0.
-      apply lt_ptr_mod in Hy.
-      unfold Ptrofs.add in *. 
+      apply lt_ptr_mod in Hy. unfold Ptrofs.add in *. 
       repeat rewrite Ptrofs.unsigned_repr_eq in *.
       rewrite Z.add_mod_idemp_r, Z.mod_small in * by easy.
       rewrite Z.mod_small; [omega|]. 
@@ -258,13 +270,22 @@ Proof.
     intuition; congruence.
 Qed.
 
+
+
+(* Verification of the function test_int_or_ptr, version 1 *)
+
+(* 
+ * This version does not include the check for (b, ofs) and (b, ofs+1).
+ * It's mostly meant to show the naive failure case.
+ *)
+
 Definition test_iop_sem : extcall_sem :=
   fun _ args m1 trc ret m2 =>
     m1 = m2 /\ trc = nil /\ 
     match args with
-    | (Vint i) :: [] =>
+    | [(Vint i)] =>
       ret = Vint (Int.modu i (Int.repr 2))
-    | (Vptr b ofs) :: [] =>
+    | [(Vptr b ofs)] =>
       ret = Vint (Ptrofs.to_int (Ptrofs.modu ofs (Ptrofs.repr 2)))
     | _ => False
     end.
@@ -274,22 +295,23 @@ Definition test_iop_sig : signature :=
 
 Lemma test_iop__extcall: extcall_properties test_iop_sem test_iop_sig.
 Proof.
-  constructor.
-  - intros. destruct H as [_ [_ ?]].
+  constructor; intros.
+  - destruct H as [_ [_ ?]].
     do 2 (destruct vargs; try destruct v; try contradiction); subst; apply I.
-  - intros. apply H0.
-  - intros. destruct H as [? _]. subst m1. trivial. 
-  - intros. destruct H as [? _]. subst m1. trivial.
-  - intros. destruct H as [? _]. subst m1. apply Mem.unchanged_on_refl.
-  - intros. exists vres, m1'.
+  - apply H0.
+  - destruct H as [? _]. subst m1. trivial. 
+  - destruct H as [? _]. subst m1. trivial.
+  - destruct H as [? _]. subst m1. apply Mem.unchanged_on_refl.
+  - exists vres, m1'.
     destruct H as [? [? ?]]. subst m2 t.
     split.
     2: split3; [apply Val.lessdef_refl | trivial | apply Mem.unchanged_on_refl]. 
     split3; trivial.
-    do 2 (destruct vargs; try destruct v; try contradiction);    
+    do 2 (destruct vargs; try destruct v; try contradiction);
       inversion H1; inversion H4; inversion H6; auto.
-  - intros. (* is the choice of f forced?? *)
-    exists f, vres, m1'. destruct H0 as [? [? ?]]; subst.
+  - (* ec_mem_inject *)
+    exists f, vres, m1'.
+    destruct H0 as [? [? ?]]; subst.
     split.
     2: {
       split.
@@ -299,12 +321,18 @@ Proof.
         split; [apply Mem.unchanged_on_refl|].
         split; [apply inject_incr_refl|].
         apply mem_lemmas.inject_separated_same_meminj.
-    } clear f H H1 H2.
+    }
     split3; trivial.
     do 2  (destruct vargs; try destruct v; try contradiction).
     + inversion H2; inversion H5; inversion H7; trivial.
     + inversion H2; inversion H5; inversion H7; subst.
-      (* dead *)
+      (* We have reason to believe that i is even, but we don't 
+       * know anything useful about delta. On the face of it, 
+       * delta need not be even. The hypothesis H1, Mem.inject, is the
+       * obvious place to look for help. I studied it carefully. 
+       * It has statements involving delta, but never comments 
+       * on delta's parity. I think we're dead.
+       *)
       admit.
   - intros. destruct H as [_ [? _]]. subst t. simpl; omega.
   - intros. generalize H. destruct H as [_ [? _]].
@@ -314,4 +342,215 @@ Proof.
     subst m1 m2 t1 t2.
     split; [constructor|]. intros _. split; trivial.
     do 2 (destruct vargs; try destruct v; try contradiction); congruence.
+Admitted.
+
+
+
+
+(* Verification of the function test_int_or_ptr, version 2 *)
+
+(* 
+ * Ref: Xavier's email on Nov 10 2018,
+ * We are checking both o and the successor of o 
+ *)
+
+Definition valid_b_o_So (m : mem) (b : block) (o : ptrofs) : Prop :=
+  Mem.perm m b (Ptrofs.unsigned o) Max Nonempty /\
+  Mem.perm m b ((Ptrofs.unsigned o) + 1) Max Nonempty.
+
+
+Lemma valid_b_o_So_dec: forall m b o, {valid_b_o_So m b o} + {~ valid_b_o_So m b o}.
+Proof.
+  intros. unfold valid_b_o_So.
+  destruct (Mem.perm_dec m b (Ptrofs.unsigned o) Max Nonempty), (Mem.perm_dec m b (Ptrofs.unsigned o + 1) Max Nonempty).
+  - left; split; trivial.
+  - right; intro; apply n; destruct H; trivial.
+  - right; intro; apply n; destruct H; trivial.
+  - right; intro. easy. 
+Qed.
+
+(* 
+ * I know this is ugly and leads to a clunky proof, but I'm just 
+ * trying to show you the computation very explicitly. 
+ * Details are in Xavier's email from November. 
+ *)
+Definition test_iop_sem' : extcall_sem :=
+  fun _ args m1 trc ret m2 =>
+    m1 = m2 /\ trc = nil /\ 
+    match args with
+    | [(Vint i)] =>
+      if (Int.eq Int.one (Int.modu i (Int.repr 2)))
+      then ret = Vone
+      else False
+    | [(Vptr b ofs)] =>
+      if (Ptrofs.eq Ptrofs.one (Ptrofs.modu ofs (Ptrofs.repr 2)))
+      then False
+      else if valid_b_o_So_dec m1 b ofs                    
+           then ret = Vzero
+           else False
+    | _ => False
+    end.
+
+Lemma test_iop__extcall': extcall_properties test_iop_sem' test_iop_sig.
+Proof.
+  constructor; intros.
+  - destruct H as [_ [_ ?]].
+    destruct vargs; try destruct v; try contradiction.
+    + destruct vargs; [|contradiction].
+      destruct (Int.eq Int.one (Int.modu i (Int.repr 2))); subst; easy.
+    + destruct vargs; [|contradiction].
+      destruct (Ptrofs.eq Ptrofs.one (Ptrofs.modu i (Ptrofs.repr 2))); [contradiction|].
+      destruct (valid_b_o_So_dec m1 b i); subst; easy.
+  - apply H0.
+  - destruct H as [? _]. subst m1. trivial. 
+  - destruct H as [? _]. subst m1. trivial.
+  - destruct H as [? _]. subst m1. apply Mem.unchanged_on_refl.
+  - destruct H as [? [? ?]]. subst m2 t.
+    exists vres, m1'. split.
+    2: split3; [apply Val.lessdef_refl | trivial | apply Mem.unchanged_on_refl].
+    split3; trivial.
+    do 2 (try destruct vargs; try destruct v); try contradiction;
+      inversion H1; inversion H4; inversion H6; auto.
+    clear -H0 H3.
+    (* 
+     * Basically we need to show that the valid_b_o_So in the hypothesis
+     * implies the valid_b_o_So in the goal. Luckily, it does. 
+     * When refactoring, I may extract this to a separate lemma, but
+     * for now I'll just strip away the details until the core goal is exposed. 
+     *)
+    destruct (Ptrofs.eq Ptrofs.one (Ptrofs.modu i (Ptrofs.repr 2))); auto.
+    destruct (valid_b_o_So_dec m1 b i); 
+      destruct (valid_b_o_So_dec m1' b i); [trivial| | contradiction..].
+    clear H3; destruct n. (* There we go, the core goal. *)
+    destruct H0 as [_ [? _ _] _]. (* And this is going to save us. *)
+    assert (inject_id b = Some (b, 0)) by now unfold inject_id.
+    unfold valid_b_o_So in *; destruct v; split.
+    + specialize (mi_perm b b 0 (Ptrofs.unsigned i) Max Nonempty H H0).
+      replace (Ptrofs.unsigned i + 0) with
+          (Ptrofs.unsigned i) in mi_perm by omega.
+      trivial.
+    + specialize (mi_perm b b 0 (Ptrofs.unsigned i + 1) Max Nonempty H H1).
+      replace (Ptrofs.unsigned i + 1 + 0) with
+          (Ptrofs.unsigned i + 1) in mi_perm by omega.
+      trivial.
+  - 
+    (** External calls must commute with memory injections,
+  in the following sense. *)
+(*  ec_mem_inject:
+    forall ge1 ge2 vargs m1 t vres m2 f m1' vargs',
+    symbols_inject f ge1 ge2 ->
+    sem ge1 vargs m1 t vres m2 ->
+    Mem.inject f m1 m1' ->
+    Val.inject_list f vargs vargs' ->
+    exists f', exists vres', exists m2',
+       sem ge2 vargs' m1' t vres' m2'
+    /\ Val.inject f' vres vres'
+    /\ Mem.inject f' m2 m2'
+    /\ Mem.unchanged_on (loc_unmapped f) m1 m2
+    /\ Mem.unchanged_on (loc_out_of_reach f m1) m1' m2'
+    /\ inject_incr f f'
+    /\ inject_separated f f' m1 m1'; 
+*)
+    intros. exists f, vres, m1'.
+    (* 
+     * A possible misstep is my choice of "f" as the meminj.
+     * I've searched the CompCert codebase for instances of "extcall properties" 
+     * being used (all of these instances are in CompCert/common/Events.v).
+     * The original f is often piped back in as the meminj in many cases.
+     * A new meminj is cooked up sometimes, 
+     * but I don't believe those cases are similar to ours.
+     * A SearchAbout on meminj shows that there aren't all that many ways to 
+     * create a new meminj... let's go on ahead for now.
+     *)
+    destruct H0 as [? [? ?]]. subst.
+    split.
+    2: {
+      split.
+      - destruct vres; auto.
+        do 2 (destruct vargs; try destruct v; try contradiction).
+        + destruct (Int.eq Int.one (Int.modu i0 (Int.repr 2))); [inversion H4 | easy]. 
+        + destruct (Ptrofs.eq Ptrofs.one (Ptrofs.modu i0 (Ptrofs.repr 2))); try contradiction.
+          destruct (valid_b_o_So_dec m2 b0 i0); [inversion H4 | easy].
+      - split; [trivial|].
+        split; [apply Mem.unchanged_on_refl|].
+        split; [apply Mem.unchanged_on_refl|].
+        split; [apply inject_incr_refl|].
+        apply mem_lemmas.inject_separated_same_meminj.
+    }
+    split3; trivial.
+    do 2 (destruct vargs; try destruct v; try contradiction).
+    + inversion H2. inversion H5. inversion H7. auto.
+    + inversion H2. inversion H5. inversion H7.
+      (* 
+       * This is where we died in version 1. 
+       * Let's keep going, we can strip away a few more layers... 
+       *)
+      subst; clear H7 H2.
+      destruct (Ptrofs.eq Ptrofs.one (Ptrofs.modu i (Ptrofs.repr 2))) eqn:parity1; [contradiction|].
+      destruct (valid_b_o_So_dec m2 b i); [|contradiction].
+      destruct (Ptrofs.eq Ptrofs.one
+                          (Ptrofs.modu (Ptrofs.add i (Ptrofs.repr delta)) (Ptrofs.repr 2))) eqn:parity2.
+      * (*
+         * From parity1 we know that i was even. 
+         * We need a contradiction from parity2.
+         
+         * By digging into Mem.inject, I can show that 
+         * delta's range is within Ptrofs.modulus.
+         * From there I can show that the Ptrofs.add in "parity2" will 
+         * work out fine and we'll just have "(i+delta) mod 2 = 1" in "parity2".
+         * For an example of this manipulation in action, 
+         * please see lines 520-529 below.
+         
+         * Anyway so after this manipulation, that we must get a 
+         * contradition from "parity2", which means showing that delta is odd.
+         * Alternately, this means showing that i and delta have opposite parities.
+         * This is the same issue we had in version 1.
+         * Again, I explored Mem.inject, which deals with delta a fair bit.
+         * Sadly, it doesn't enforce anything about delta's parity.
+         * I think we're dead once again.
+         *)
+        admit. 
+      * destruct (valid_b_o_So_dec m1' b2 (Ptrofs.add i (Ptrofs.repr delta))); auto.
+        destruct n.
+        destruct H1 as [[? _ _] _ _ _ rep _].
+        clear - mi_perm v H10 rep.
+        unfold valid_b_o_So in *.
+        destruct v; split.
+        -- specialize (mi_perm _ _ _ (Ptrofs.unsigned i) Max Nonempty H10 H).
+           replace (Ptrofs.unsigned (Ptrofs.add i (Ptrofs.repr delta))) with
+               (Ptrofs.unsigned i + delta).
+           2: {
+             destruct (rep _ _ delta i H10).
+             1: left; trivial. 
+             unfold Ptrofs.add.
+             repeat rewrite Ptrofs.unsigned_repr_eq.
+             rewrite Z.add_mod_idemp_r by easy.
+             apply lt_ptr_mod in H2. 
+             rewrite Z.mod_small by easy. trivial. 
+           }
+           trivial.
+        -- specialize (mi_perm _ _ _ (Ptrofs.unsigned i + 1) Max Nonempty H10 H0).
+           replace (Ptrofs.unsigned (Ptrofs.add i (Ptrofs.repr delta)) + 1) with (Ptrofs.unsigned i + 1 + delta).
+            2: {
+              destruct (rep _ _ delta i H10).
+              left; trivial. 
+              unfold Ptrofs.add.
+              repeat rewrite Ptrofs.unsigned_repr_eq.
+              rewrite Z.add_mod_idemp_r by easy.
+              apply lt_ptr_mod in H2.
+              rewrite Z.mod_small by easy. omega.
+            }
+            trivial.
+  - destruct H as [_ [? _]]. subst t. simpl; omega.
+  - generalize H. destruct H as [_ [? _]].
+    subst t1; inversion H0; subst t2.
+    intro H; exists vres1, m1; apply H.
+  - destruct H as [? [? ?]]. destruct H0 as [? [? ?]].
+    subst m1 m2 t1 t2.
+    split; [constructor|]. intros _. split; trivial.
+    do 2 (try destruct vargs; try destruct v; try contradiction).
+    + destruct (Int.eq Int.one (Int.modu i (Int.repr 2))); subst; [trivial | contradiction].
+    + destruct (Ptrofs.eq Ptrofs.one (Ptrofs.modu i (Ptrofs.repr 2))); [contradiction|].      
+      destruct (valid_b_o_So_dec m b i); [|contradiction].
+      subst; trivial.
 Admitted.
